
# Some thing about the *Fixed-point Combinators* 

## И SKI

### Knows

We have:

~~~ lambda
S = 位abc.ac(bc)
K = 位ab.a = 位xy.x
I = 位a.a
~~~

and 

~~~ lambda
Y = 位f.(位s.ss)(位x.f(xx))
~~~

And that's what I want to prove: 

~~~ lambda
Y = S(K(SII))(S(S(KS)K)(K(SII)))
~~~

### Provings

~~~ lambda
SII = 位c.c(c) = 位s.ss = M
KM = 位ab.bb = 位xy.yy
KS = 位xabc.ac(bc)

S(KS)
 = 位bc.(位xa'b'c'.a'c'(b'c'))c(bc)
 = 位bc.(位b'c'.bcc'(b'c'))
 = 位bcde.bce(de)

S(KS)K = 位cde.c(de) = B = 位xyz.x(yz)
SB = 位bcz.c(bcz) = 位xyz.y(xyz)
SB(KM) = 位yz.y(zz) = 位ab.a(bb) = L
S(KM) = 位bc.(bc)(bc) = 位ab.ab(ab) = M2

S(KM)L
 = 位b. (位yz.y(zz))b ((位yz.y(zz))b)
 = 位b. (位z.b(zz)) ((位yz.y(zz))b)
 = 位b. (位z.b(zz)) (位z.b(zz)) = 位f. (位x.f(xx)) (位x.f(xx)) = Y
~~~

So: 

~~~ lambda
Y = S(KM)L
 = 位f.(位x.f(xx))(位x.f(xx))
 = 位f.M(位x.f(xx))
 = 位f.(位s.ss)(位x.f(xx))
~~~

So we can sure: 

~~~ lambda
Y
 = S(K(SII))(S(S(KS)K)(K(SII)))
 = S(K(M))(S(S(KS)K)(K(M)))
 = S(KM)(SB(KM))
 = S(KM)L = 位f.(位x.f(xx))(位x.f(xx))
~~~

### More

And that is how the `Y` works:

~~~ lambda
Y = S(KM)L
 = 位b. (位z.b(zz)) (位z'.b(z'z'))
 = 位b. (b( (位z'.b(z'z')) (位z'.b(z'z')) ))
 = 位b. (b( (位z'.b(z'z')) (位z''.b(z''z'')) ))
 = 位b. b b ( (位z''.b(z''z'')) (位z''.b(z''z'')) )
 = 位b. b b ( (位z''.b(z''z'')) (位z'.b(z'z')) )
 = 位b. b b b ( (位z'.b(z'z')) (位z''.b(z''z'')) )
 = 位b. b b b b ( (位z''.b(z''z'')) (位z'.b(z'z')) )
 = 位b. b b b b b ( (位z'.b(z'z')) (位z''.b(z''z'')) )
 = 位b. b b b b b b ( (位z''.b(z''z'')) (位z'.b(z'z')) )
 ...
~~~


##  Y & Z

We know: 

~~~ lambda
Y = 位f.(位s.ss)(位x.f(xx))
Z = 位f.(位s.ss)(位x.f(位z.(xx)z))
~~~

### Same

And for all combinator `F` and `X`, the `(位z. F z) X` is just equal with `F X`, this is just by the ***尾-reduction***.

So: for all combinator `F`, the `(位z. F z)` is just equal with `F`. Means, `位x.f(位z.(xx)z)` just same as `位x.f(xx)`.

So we can know that, a `Z` is just a `Y`.

### Diff

**But**, if your compute system is not like the form system of *lambda-calculus*, you may need to use `Z` not `Y`. That's because even they are same thing in *lambda-calculus*, they're also able to use for declare different behavior in other system and that's only need there shall have different behavior between `xx` and `位z.(xx)z` in that compute system.

That's why there's also a `Z`, not only a `Y`, or things won't be enough.

Such as `位z.(xx)z` is just means a value, but `xx` means make a *evaluate* in time and immediately. You can found such design of these behaviors in most of computer programming languages.

- Such as `(x) (x)` in *JS* means there will make a evaluate in time so the `Y` must make a *stack overflow* error. Here, you must replace the `(x) (x)` with a `z => (x) (x) (z)` namely that means replace `Y` with `Z`.
- But a same `(x) (x)` in *Lua* can just means a value until it need be evaluated, so even the `(function (x) return (x) (x) end) (function (x) return (x) (x) end)` also won't make any error. And if you want to told the computer it should be evaluate in time in *Lua*, you just write a `((x) (x))` then it will evaluated immediately, so you can just write a `(function (x) return ((x) (x)) end) (function (x) return ((x) (x)) end)` to *Lua* to get a *stack overflow* error.

##  And

### *SK*

The simplest fixed-point combinator in the SK-calculus (found by [John Tromp](https://en.wikipedia.org/wiki/John_Tromp 'John Tromp is a Dutch computer scientist. He formerly worked for Dutch Centre for Mathematics and Computer Science. Tromp discovered the number of legal states of the board game Go, and co-authored with Bill Taylor the Tromp-Taylor Rules, which they call "the logical rules of Go". He is also known for Binary combinatory logic (Binary lambda calculus).')) and its corresponds to the lambda expression is: 

~~~ ml
Y' = SSK(S(K(SS(S(SSK))))K)
Y' = (位ab.aba) (位ab.a(bab))
~~~

Provings: 

~~~ ml
Y' = SSK(S(K(SS(S(SSK))))K)

S = 位abc.ac(bc)
K = 位ab.a

SS 
 = (位abc.ac(bc)) (位a'b'c'.a'c'(b'c'))
 = (位bc.(位a'b'c'.a'c'(b'c'))c(bc))
 = (位bc.(位c'.cc'((bc)c')))
 = (位abc.bc(abc))

SSK 
 = (位abc.bc(abc)) (位a'b'.a')
 = (位bc.bc((位a'b'.a')bc))
 = (位bc.bc(b))
 = (位ab.aba)

SSK 
 = (位abc.ac(bc)) (位abc.ac(bc)) (位ab.a)
 = (位abc.ac(bc)) (位a'b'c'.a'c'(b'c')) (位a''b''.a'')
 = (位c.(位a'b'c'.a'c'(b'c'))c((位a''b''.a'')c))
 = (位c.(位b'c'.cc'(b'c'))(位b''.c))
 = (位c.(位c'.cc'((位b''.c)c')))
 = (位c.(位c'.cc'c))
 = (位ab.aba)

S(SSK) 
 = (位abc.ac(bc)) (位a'b'.a'b'a')
 = (位bc.(位a'b'.a'b'a')c(bc))
 = (位bc.(位b'.cb'c)(bc))
 = (位bc.(c(bc)c))
 = (位ab.b(ab)b)

SS(S(SSK)) 
 = (位abc.bc(abc)) (位a'b'.b'(a'b')b')
 = (位bc.bc((位a'b'.b'(a'b')b')bc))
 = (位bc.bc((c(bc)c)))
 = (位ab.ab(b(ab)b))

K(SS(S(SSK))) 
 = (位a'b'.a') (位ab.ab(b(ab)b))
 = (位b'.(位ab.ab(b(ab)b)))
 = (位a.(位bc.bc(c(bc)c)))
 = (位abc.bc(c(bc)c))

S(K(SS(S(SSK)))) 
 = (位abc.ac(bc)) (位a'b'c'.b'c'(c'(b'c')c'))
 = (位bc.(位a'b'c'.b'c'(c'(b'c')c'))c(bc))
 = (位bc.(位c'.(bc)c'(c'((bc)c')c')))
 = (位ab.位c.(ab)c(c((ab)c)c))
 = (位abc.abc(c(abc)c))

S(K(SS(S(SSK))))K 
 = (位abc.abc(c(abc)c)) (位a'b'.a')
 = (位bc.(位a'b'.a')bc(c((位a'b'.a')bc)c))
 = (位bc.b(c(b)c))
 = (位ab.a(bab))

SSK(S(K(SS(S(SSK))))K) 
 = (位a'b'.a'b'a') (位ab.a(bab))
 = (位b'.(位ab.a(bab))b'(位ab.a(bab)))
 = (位b'.(位b.b'(bb'b))(位ab.a(bab)))
 = (位b'.(b'((位ab.a(bab))b'(位ab.a(bab)))))
 = (位b'.(b'((位b.b'(bb'b))(位ab.a(bab)))))
 = (位b'.(b'((b'((位ab.a(bab))b'(位ab.a(bab)))))))
 = (位b'.(b'(b'((位ab.a(bab))b'(位ab.a(bab))))))
 = (位b'.(b'(b'(b'((位ab.a(bab))b'(位ab.a(bab)))))))
 = (位b'.(b'(b'(b'(b'((位ab.a(bab))b'(位ab.a(bab))))))))
 = ...
 = (位a'b'.a'b'a') (位ab.a(bab))
 = (位ab.aba) (位ab.a(bab))

Y' = SSK(S(K(SS(S(SSK))))K) = (位ab.aba) (位ab.a(bab))
~~~

### *Turing fixed-point combinator*

~~~ ml
 = (位ab.b(aab)) (位ab.b(aab)) = (位x.xx) (位ab.b(aab))
~~~

~~~ ml
 = (位ab.b(aab)) (位ab.b(aab)) = (位x.xx) (位ab.b(aab))

(位ab.b(aab)) (位ab.b(aab)) 
 = (位a''b''.b''(a''a''b'')) (位ab.b(aab))
 = (位b''.b''((位a'b'.b'(a'a'b'))(位ab.b(aab))b''))
 = (位b''.b''((位b'.b'((位ab.b(aab))(位ab.b(aab))b'))b''))
 = (位b'''.b'''((位b''.b''((位a'b'.b'(a'a'b'))(位ab.b(aab))b''))b'''))
 = (位b'''.b'''((位b''.b''((位b'.b'((位ab.b(aab))(位ab.b(aab))b'))b''))b'''))
 = (位b'''.b'''((b'''((位b'.b'((位ab.b(aab))(位ab.b(aab))b'))b'''))))
 = (位b'''.b'''((b'''((b'''((位ab.b(aab))(位ab.b(aab))b'''))))))
 = (位b'''.b'''(b'''(b'''((位ab.b(aab))(位ab.b(aab))b'''))))
 = (位t.t(t(t((位ab.b(aab))(位ab.b(aab))t))))
 = (位t.t(t(t(t((位ab.b(aab))(位ab.b(aab))t)))))
 = (位t.t(t(t(t(t((位ab.b(aab))(位ab.b(aab))t))))))
 = (位t.t(t(t(t(t(t((位ab.b(aab))(位ab.b(aab))t)))))))
 = (位t.t(t(t(t(t(t(t)))))))
 = (位t.t(t(t(t(t(t(t(t))))))))
 = ...

t = t(t)
~~~

~~~ ml
A' = 位z.Az
A' a 
 = (位z.Az) a
 = A a

位z.Az 
 = A'
 = A

 
 = (位x.xx) (位ab.b(aab))
 = (位x.xx) (位ab.b(位z.aabz))
~~~

### *Another type of 'Z'*

~~~ ml
Z  = 位f.(位s.ss)(位x.f(位z.(xx)z))
Z' = 位f.(位s.ss)(位x.位z.f((xx)z))
~~~

`Z` is simply equal to `Y`: 

~~~ ml
A' = 位z.Az
A' a 
 = (位z.Az) a
 = A a

位z.Az 
 = A'
 = A

Z 
 = 位f.(位s.ss)(位x.f(位z.(xx)z))
 = 位f.(位s.ss)(位x.f(xx))
 = Y
~~~

`Z'`: 

~~~ ml
Z' 
 = 位f.(位s.ss)(位x.位z.f((xx)z))
 = 位f.(位xz.f((xx)z))(位xz.f((xx)z))

Z' f 
 = (位f.(位xz.f((xx)z))(位xz.f((xx)z))) f
 = (位xz.f((xx)z)) (位xz.f((xx)z))

Z' 
 = 位f.(位xz.f((xx)z))(位xz.f((xx)z))
 = 位f.(位z'.f(((位xz.f((xx)z))(位xz.f((xx)z)))z'))
 = 位fg.f(((位xz.f((xx)z)) (位xz.f((xx)z)))g)
 = 位fg.f((Z' f)g)
 = 位fg.f(Z'fg)
 = 位fg.f((位f'g'.f'(Z'f'g'))fg)
 = 位fg.f(f(Z'fg))
 = 位fg.f(f(f(Z'fg)))
 = 位fg.f(f(f(f(Z'fg))))
 = ...

Z' a b 
 = (位fg.f(Z'fg)) a b
 = (a (Z' a b))
 = (a (a (Z' a b)))
 = (a (a (a (Z' a b))))
 = ...

Z' a b = (a (Z' a b))
~~~



##  Also

- <sup>([BCL](https://en.wikipedia.org/wiki/Binary_combinatory_logic "Binary combinatory logic"))</sup> Binary combinatory logic
- <sup>([IAJ](https://en.wikipedia.org/wiki/Iota_and_Jot "Iota and Jot"))</sup> Iota and Jot
- <sup>([SKI](https://en.wikipedia.org/wiki/SKI_combinator_calculus "SKI combinator calculus"))</sup> SKI combinator calculus
- <sup>([UNL](https://en.wikipedia.org/wiki/Unlambda "Unlambda"))</sup> Unlambda
- <sup>([LZK](https://tromp.github.io/cl/lazy-k.html "Lazy-K"))</sup> Lazy-K
- <sup>([TCP](https://esolangs.org/wiki/S_and_K_Turing-completeness_proof "S and K Turing-completeness proof"))</sup> S and K Turing-completeness proof

